proofmode/class_instances.v
@@ -275,17 +275,17 @@ Proof.
   rewrite /Frame /MakeLater=><- <-. by rewrite later_sep -(later_intro R).
 Qed.
 
-Class MakeNowTrue (P Q : uPred M) := make_now_True : ◇ P ⊣⊢ Q.
-Global Instance make_now_True_True : MakeNowTrue True True.
-Proof. by rewrite /MakeNowTrue now_True_True. Qed.
-Global Instance make_now_True_default P : MakeNowTrue P (◇ P) | 100.
+Class MakeNowTrue (P Q : uPred M) := make_except_now : ◇ P ⊣⊢ Q.
+Global Instance make_except_except_now : MakeNowTrue True True.
+Proof. by rewrite /MakeNowTrue except_except_now. Qed.
+Global Instance make_except_now_default P : MakeNowTrue P (◇ P) | 100.
 Proof. done. Qed.
 
-Global Instance frame_now_true R P Q Q' :
+Global Instance frame_except_now R P Q Q' :
   Frame R P Q → MakeNowTrue Q Q' → Frame R (◇ P) Q'.
 Proof.
   rewrite /Frame /MakeNowTrue=><- <-.
-  by rewrite now_True_sep -(now_True_intro R).
+  by rewrite except_now_sep -(except_now_intro R).
 Qed.
 
 Global Instance frame_exist {A} R (Φ Ψ : A → uPred M) :
@@ -332,20 +332,20 @@ Global Instance into_exist_always {A} P (Φ : A → uPred M) :
 Proof. rewrite /IntoExist=> HP. by rewrite HP always_exist. Qed.
 
 (* IntoNowTrue *)
-Global Instance into_now_True_now_True P : IntoNowTrue (◇ P) P.
+Global Instance into_except_now_except_now P : IntoNowTrue (◇ P) P.
 Proof. done. Qed.
-Global Instance into_now_True_timeless P : TimelessP P → IntoNowTrue (▷ P) P.
+Global Instance into_except_now_timeless P : TimelessP P → IntoNowTrue (▷ P) P.
 Proof. done. Qed.
 
 (* IsNowTrue *)
-Global Instance is_now_True_now_True P : IsNowTrue (◇ P).
-Proof. by rewrite /IsNowTrue now_True_idemp. Qed.
-Global Instance is_now_True_later P : IsNowTrue (▷ P).
-Proof. by rewrite /IsNowTrue now_True_later. Qed.
-Global Instance is_now_True_rvs P : IsNowTrue P → IsNowTrue (|=r=> P).
+Global Instance is_except_now_except_now P : IsNowTrue (◇ P).
+Proof. by rewrite /IsNowTrue except_now_idemp. Qed.
+Global Instance is_except_now_later P : IsNowTrue (▷ P).
+Proof. by rewrite /IsNowTrue except_now_later. Qed.
+Global Instance is_except_now_rvs P : IsNowTrue P → IsNowTrue (|=r=> P).
 Proof.
   rewrite /IsNowTrue=> HP.
-  by rewrite -{2}HP -(now_True_idemp P) -now_True_rvs -(now_True_intro P).
+  by rewrite -{2}HP -(except_now_idemp P) -except_now_rvs -(except_now_intro P).
 Qed.
 
 (* FromViewShift *)
