proofmode/classes.v
@@ -55,11 +55,11 @@ Class IntoExist {A} (P : uPred M) (Φ : A → uPred M) :=
   into_exist : P ⊢ ∃ x, Φ x.
 Global Arguments into_exist {_} _ _ {_}.
 
-Class IntoNowTrue (P Q : uPred M) := into_now_True : P ⊢ ◇ Q.
-Global Arguments into_now_True : clear implicits.
+Class IntoNowTrue (P Q : uPred M) := into_except_now : P ⊢ ◇ Q.
+Global Arguments into_except_now : clear implicits.
 
-Class IsNowTrue (Q : uPred M) := is_now_True : ◇ Q ⊢ Q.
-Global Arguments is_now_True : clear implicits.
+Class IsNowTrue (Q : uPred M) := is_except_now : ◇ Q ⊢ Q.
+Global Arguments is_except_now : clear implicits.
 
 Class FromVs (P Q : uPred M) := from_vs : (|=r=> Q) ⊢ P.
 Global Arguments from_vs : clear implicits.
